Update syntax

theories/Syntax.v
@@ -28,16 +28,12 @@ Inductive exp : Set :=
   | a_app : exp -> exp -> exp
   | a_pi : exp -> exp -> exp
   (* Substitutions *)
-  | a_sub : exp -> subst -> exp
-with subst : Set :=
-  | a_id : subst
-  | a_weaken : subst
-  | a_compose : subst -> subst -> subst
-  | a_extend : subst -> exp -> subst.
-
-(* Some convenient infix notations *)
-Infix "∙" := a_compose (at level 70).
-Infix ",," := a_extend (at level 80).
+  | a_sub : exp -> sub -> exp
+with sub : Set :=
+  | a_id : sub
+  | a_weaken : sub
+  | a_compose : sub -> sub -> sub
+  | a_extend : sub -> exp -> sub.
 
 Fixpoint nat_to_exp n : exp :=
   match n with
@@ -66,32 +62,33 @@ Definition exp_to_num e :=
 #[global] Declare Scope exp_scope.
 #[global] Delimit Scope exp_scope with exp.
 #[global] Bind Scope exp_scope with exp.
-#[global] Bind Scope exp_scope with subst.
+#[global] Bind Scope exp_scope with sub.
+#[global] Bind Scope exp_scope with Sortclass.
 Open Scope exp_scope.
 Open Scope nat_scope.
 
-Notation "<{ x }>" := x (at level 0, x custom exp at level 99) : exp_scope.
-Notation "( x )" := x (in custom exp at level 0, x custom exp at level 99) : exp_scope.
-Notation "~{ x }" := x (in custom exp at level 0, x constr at level 0) : exp_scope.
+Notation "{{{ x }}}" := x (at level 0, x custom exp at level 99, format "'{{{'  x  '}}}'") : exp_scope.
+Notation "( x )" := x (in custom exp at level 0, x custom exp at level 60) : exp_scope.
+Notation "~ x" := x (in custom exp at level 0, x constr at level 0) : exp_scope.
 Notation "x" := x (in custom exp at level 0, x constr at level 0) : exp_scope.
-Notation "e |[ s ]|" := (a_sub e s) (in custom exp at level 0, s custom exp at level 99) : exp_scope.
+Notation "e [ s ]" := (a_sub e s) (in custom exp at level 0, s custom exp at level 60) : exp_scope.
 Notation "'λ' T e" := (a_fn T e) (in custom exp at level 0, T custom exp at level 30, e custom exp at level 30) : exp_scope.
 Notation "f x .. y" := (a_app .. (a_app f x) .. y) (in custom exp at level 40, f custom exp, x custom exp at next level, y custom exp at next level) : exp_scope.
 Notation "'ℕ'" := a_nat (in custom exp) : exp_scope.
-Notation "'Type(' n ')'" := (a_typ n) (in custom exp at level 0, n constr at level 99) : exp_scope.
+Notation "'Type' @ n" := (a_typ n) (in custom exp at level 0, n constr at level 0) : exp_scope.
 Notation "'Π' T S" := (a_pi T S) (in custom exp at level 0, T custom exp at level 30, S custom exp at level 30) : exp_scope.
 Number Notation exp num_to_exp exp_to_num : exp_scope.
-Notation "'suc' e" := (a_succ e) (in custom exp at level 30, e custom exp at level 30) : exp_scope.
+Notation "'zero'" := a_zero (in custom exp at level 0) : exp_scope.
+Notation "'succ' e" := (a_succ e) (in custom exp at level 30, e custom exp at level 30) : exp_scope.
 Notation "'#' n" := (a_var n) (in custom exp at level 0, n constr at level 0) : exp_scope.
 Notation "'Id'" := a_id (in custom exp at level 0) : exp_scope.
 Notation "'Wk'" := a_weaken (in custom exp at level 0) : exp_scope.
-Infix "∙" := a_compose (in custom exp at level 70) : exp_scope.
-Infix "," := a_extend (in custom exp at level 80) : exp_scope.
 
-Notation Ctx := (list exp).
-Notation Sb := subst.
-Notation Typ := exp.
-Notation typ := a_typ.
-Notation ℕ := a_nat.
-Notation 𝝺 := a_fn.
-Notation Π := a_pi.
+Notation "⋅" := nil (in custom exp at level 0) : exp_scope.
+Notation "x , y" := (cons y x) (in custom exp at level 50) : exp_scope.
+
+Infix "∘" := a_compose (in custom exp at level 40) : exp_scope.
+Infix ",," := a_extend (in custom exp at level 50) : exp_scope.
+
+Notation ctx := (list exp).
+Notation typ := exp.
