theories/CtxEqLemmas.v
@@ -3,26 +3,26 @@ Require Import Mcltt.Syntax.
 Require Export Mcltt.System.
 Require Export Mcltt.LibTactics.
 
-Lemma ctx_decomp : forall {Γ T}, ⊢ T :: Γ -> (⊢ Γ ∧ ∃ i, Γ ⊢ T : typ i).
+Lemma ctx_decomp : forall {Γ T}, {{ ⊢ Γ , T }} -> {{ ⊢ Γ }} ∧ ∃ i, {{ Γ ⊢ T : Type@i }}.
 Proof with mauto.
   intros * HTΓ.
   inversion HTΓ; subst...
 Qed.
 
 (* Corresponds to presup-⊢≈ in the Agda proof *)
-Lemma presup_ctx_eq : forall {Γ Δ}, ⊢ Γ ≈ Δ -> ⊢ Γ ∧ ⊢ Δ.
+Lemma presup_ctx_eq : forall {Γ Δ}, {{ ⊢ Γ ≈ Δ }} -> {{ ⊢ Γ }} ∧ {{ ⊢ Δ }}.
 Proof with mauto.
   intros * HΓΔ.
   induction HΓΔ as [|* ? [? ?]]...
 Qed.
 
-(* Corresponds to ≈-refl in the Agda code*)
-Lemma tm_eq_refl : forall {Γ t T}, Γ ⊢ t : T -> Γ ⊢ t ≈ t : T.
+(* Corresponds to ≈-refl in the Agda code *)
+Lemma tm_eq_refl : forall {Γ t T}, {{ Γ ⊢ t : T }} -> {{ Γ ⊢ t ≈ t : T }}.
 Proof.
   mauto.
 Qed.
 
-Lemma sb_eq_refl : forall {Γ Δ σ}, Γ ⊢s σ : Δ -> Γ ⊢s σ ≈ σ : Δ.
+Lemma sb_eq_refl : forall {Γ Δ σ}, {{ Γ ⊢s σ : Δ }} -> {{ Γ ⊢s σ ≈ σ : Δ }}.
 Proof.
   mauto.
 Qed.
@@ -31,22 +31,22 @@ Qed.
 Hint Resolve ctx_decomp presup_ctx_eq tm_eq_refl sb_eq_refl : mcltt.
 
 (* Corresponds to t[σ]-Se in the Agda proof *)
-Lemma sub_lvl : forall {Δ Γ T σ i}, Δ ⊢ T : typ i -> Γ ⊢s σ : Δ -> Γ ⊢ a_sub T σ : typ i.
+Lemma exp_sub_typ : forall {Δ Γ T σ i}, {{ Δ ⊢ T : Type@i }} -> {{ Γ ⊢s σ : Δ }} -> {{ Γ ⊢ T[σ] : Type@i }}.
 Proof.
   mauto.
 Qed.
 
 (* Corresponds to []-cong-Se′ in the Agda proof*)
-Lemma sub_lvl_eq : forall {Δ Γ T T' σ i}, Δ ⊢ T ≈ T' : typ i -> Γ ⊢s σ : Δ -> Γ ⊢ a_sub T σ ≈ a_sub T' σ : typ i.
+Lemma eq_exp_sub_typ : forall {Δ Γ T T' σ i}, {{ Δ ⊢ T ≈ T' : Type@i }} -> {{ Γ ⊢s σ : Δ }} -> {{ Γ ⊢ T[σ] ≈ T'[σ] : Type@i }}.
 Proof.
   mauto.
 Qed.
 
 #[export]
-Hint Resolve sub_lvl sub_lvl_eq : mcltt.
+Hint Resolve exp_sub_typ eq_exp_sub_typ : mcltt.
 
 (* Corresponds to ∈!⇒ty-wf in Agda proof *)
-Lemma var_in_wf : forall {Γ T x}, ⊢ Γ -> x : T ∈! Γ -> ∃ i, Γ ⊢ T : typ i.
+Lemma var_in_wf : forall {Γ T x}, {{ ⊢ Γ }} -> {{ #x : T ∈ Γ }} -> ∃ i, {{ Γ ⊢ T : Type@i }}.
 Proof with mauto.
   intros * HΓ Hx. gen x T.
   induction HΓ; intros; inversion_clear Hx as [|? ? ? ? Hx']...
@@ -56,7 +56,7 @@ Qed.
 #[export]
 Hint Resolve var_in_wf : mcltt.
 
-Lemma presup_sb_ctx : forall {Γ Δ σ}, Γ ⊢s σ : Δ -> ⊢ Γ ∧ ⊢ Δ.
+Lemma presup_sb_ctx : forall {Γ Δ σ}, {{ Γ ⊢s σ : Δ }} -> {{ ⊢ Γ }} ∧ {{ ⊢ Δ }}.
 Proof with mauto.
   intros * Hσ.
   induction Hσ...
@@ -70,7 +70,7 @@ Qed.
 #[export]
 Hint Resolve presup_sb_ctx : mcltt.
 
-Lemma presup_tm_ctx : forall {Γ t T}, Γ ⊢ t : T -> ⊢ Γ.
+Lemma presup_tm_ctx : forall {Γ t T}, {{ Γ ⊢ t : T }} -> {{ ⊢ Γ }}.
 Proof with mauto.
   intros * Ht.
   induction Ht...
@@ -81,7 +81,7 @@ Qed.
 Hint Resolve presup_tm_ctx : mcltt.
 
 (* Corresponds to ∈!⇒ty≈ in Agda proof *)
-Lemma var_in_eq : forall {Γ Δ T x}, ⊢ Γ ≈ Δ -> x : T ∈! Γ -> ∃ S i, x : S ∈! Δ ∧ Γ ⊢ T ≈ S : typ i ∧ Δ ⊢ T ≈ S : typ i.
+Lemma var_in_eq : forall {Γ Δ T x}, {{ ⊢ Γ ≈ Δ }} -> {{ #x : T ∈ Γ }} -> ∃ S i, {{ #x : S ∈ Δ }} ∧ {{ Γ ⊢ T ≈ S : Type@i }} ∧ {{ Δ ⊢ T ≈ S : Type@i }}.
 Proof with mauto.
   intros * HΓΔ Hx.
   gen Δ; induction Hx; intros; inversion_clear HΓΔ as [|? ? ? ? ? HΓΔ'].
@@ -91,7 +91,7 @@ Proof with mauto.
 Qed.
 
 (* Corresponds to ⊢≈-sym in Agda proof *)
-Lemma ctx_eq_sym : forall {Γ Δ}, ⊢ Γ ≈ Δ -> ⊢ Δ ≈ Γ.
+Lemma ctx_eq_sym : forall {Γ Δ}, {{ ⊢ Γ ≈ Δ }} -> {{ ⊢ Δ ≈ Γ }}.
 Proof with mauto.
   intros.
   induction H...
@@ -100,7 +100,7 @@ Qed.
 #[export]
 Hint Resolve var_in_eq ctx_eq_sym : mcltt.
 
-Lemma presup_sb_eq_ctx : forall {Γ Δ σ σ'}, Γ ⊢s σ ≈ σ' : Δ -> ⊢ Γ.
+Lemma presup_sb_eq_ctx : forall {Γ Δ σ σ'}, {{ Γ ⊢s σ ≈ σ' : Δ }} -> {{ ⊢ Γ }}.
 Proof with mauto.
   intros.
   induction H; mauto; now (eapply proj1; mauto).
@@ -109,12 +109,12 @@ Qed.
 #[export]
 Hint Resolve presup_sb_eq_ctx : mcltt.
 
-Lemma presup_tm_eq_ctx : forall {Γ t t' T}, Γ ⊢ t ≈ t' : T -> ⊢ Γ.
+Lemma presup_tm_eq_ctx : forall {Γ t t' T}, {{ Γ ⊢ t ≈ t' : T }} -> {{ ⊢ Γ }}.
 Proof with mauto.
   intros.
   induction H...
   Unshelve.
-  exact 0%nat.
+  constructor.
 Qed.
 
 #[export]
